may break OCaml

coq/Word/WordInterface.v
@@ -4,6 +4,7 @@ Require Import Coq.Logic.ProofIrrelevance.
 Require Import Coq.Structures.Equalities.
 Require Import PArith.BinPos.
 Require Import NArith.BinNat.
+Require Import Bag.TotalOrder.
 
 Local Open Scope N_scope.
 
@@ -43,8 +44,94 @@ Module MakeWord (Width : WIDTH).
 
   Definition zero : t := @Mk 0 eq_refl.
 
-End MakeWord.
+  Lemma eq_dec : forall (m n : t), { m = n } + { m <> n }.
+  Proof.
+    intros.
+    destruct m, n.
+    assert ({v = v0} + {v <> v0}) as J.
+    { apply N.eq_dec. }
+    destruct J; subst.
+    + left.
+      f_equal.
+      apply proof_irrelevance.
+    + right.
+      unfold not.
+      intros.
+      inversion H; subst.
+      contradiction n.
+      reflexivity.
+  Qed.
 
+  Definition le (x y : t) : Prop :=
+    match (x, y) with
+      | (Mk m _, Mk n _) => m <= n
+    end.
+
+  Lemma le_reflexivity : forall (x : t), le x x.
+  Proof with auto.
+    intros.
+    destruct x...
+    apply N.le_refl.
+  Qed.
+
+  Lemma le_antisymmetry : forall (x y : t), le x y -> le y x -> x = y.
+  Proof with eauto.
+    intros.
+    destruct x, y.
+    unfold le in *.
+    apply N.lt_eq_cases in H.
+    apply N.lt_eq_cases in H0.
+    destruct H, H0...
+    + assert (v < v). eapply N.lt_trans...
+      apply N.lt_irrefl in H1. inversion H1.
+    + subst...
+      assert (l = l0). apply proof_irrelevance.
+      subst...
+    + subst...
+      assert (l = l0). apply proof_irrelevance.
+      subst...
+    + clear H0; subst.
+      assert (l = l0). apply proof_irrelevance.
+      subst...
+  Qed.
+
+  Lemma le_transitivity : forall (x y z : t), le x y -> le y z -> le x z.
+  Proof with eauto.
+    intros.
+    destruct x, y, z.
+    unfold le in *.
+    eapply N.le_trans...
+  Qed.
+
+  Lemma le_compare : forall (x y : t), { le x y } + { le y x }.
+  Proof with eauto.
+    intros.
+    destruct x, y.
+    unfold le in *.
+    remember (N.compare v v0) as cmp eqn:J.
+    symmetry in J.
+    destruct cmp.
+    + apply N.compare_eq_iff in J.
+      subst.
+      left...
+      apply N.lt_eq_cases...
+    + rewrite ->  N.compare_lt_iff in J.
+      left.
+      apply N.lt_eq_cases...
+    + rewrite ->  N.compare_gt_iff in J.
+      right.
+      apply N.lt_eq_cases...
+  Qed.
+ 
+  Instance TotalOrder :  TotalOrder le := {
+    reflexivity := le_reflexivity;
+    antisymmetry := le_antisymmetry;
+    transitivity := le_transitivity;
+    compare := le_compare;
+    eqdec := eq_dec
+  }.
+
+End MakeWord.
 
 Module Width8 <: WIDTH.
 
@@ -93,16 +180,12 @@ Module Word8 <: WORD.
   Module M := MakeWord (Width8).
   Include M.
 
-  Parameter eq_dec : forall (m n : t), { m = n } + { m <> n }.
-
 End Word8.
 
 Module Word12 <: WORD.
 
   Module M := MakeWord (Width12).
   Include M.
-
-  Parameter eq_dec : forall (m n : t), { m = n } + { m <> n }.
 
 End Word12.
 
@@ -122,25 +205,18 @@ Module Word16 <: WORD.
   (* TODO(arjun): broken now for simplicity *)
   Axiom pred : Word -> Word.
 
-  Parameter eq_dec : forall (m n : t), { m = n } + { m <> n }.
-
 End Word16.
 
 Module Word32 <: WORD.
 
   Module M := MakeWord (Width32).
   Include M.
-
-  Parameter eq_dec : forall (m n : t), { m = n } + { m <> n }.
-
 End Word32.
 
 Module Word48 <: WORD.
 
   Module M := MakeWord (Width48).
   Include M.
-
-  Parameter eq_dec : forall (m n : t), { m = n } + { m <> n }.
 
 End Word48.
 
@@ -149,9 +225,10 @@ Module Word64 <: WORD.
   Module M := MakeWord (Width64).
   Include M.
 
-  Parameter eq_dec : forall (m n : t), { m = n } + { m <> n }.
-
 End Word64.
+
+Existing Instances Word8.TotalOrder Word16.TotalOrder Word12.TotalOrder
+  Word32.TotalOrder Word48.TotalOrder Word64.TotalOrder.
 
 Extract Constant Word16.pred => "(fun n -> if n = 0 then 0 else n - 1)". (* TODO: really fix this (JNF) *)
 Extract Constant Word16.max_value => "65535".
@@ -176,3 +253,9 @@ Extract Constant Word16.zero => "0".
 Extract Constant Word32.zero => "Int32.zero".
 Extract Constant Word48.zero => "Int64.zero".
 Extract Constant Word64.zero => "Int64.zero".
+
+Extract Constant Word8.le_compare => "(<=)".
+Extract Constant Word16.le_compare => "(<=)".
+Extract Constant Word32.le_compare => "(fun x y -> Int32.compare x y <= 0)".
+Extract Constant Word48.le_compare => "(fun x y -> Int64.compare x y <= 0)".
+Extract Constant Word64.le_compare => "(fun x y -> Int64.compare x y <= 0)".
