coq/Bag/TotalOrder.v
@@ -295,3 +295,10 @@ Extract Constant TotalOrder_pair =>
 "fun _ _ -> { compare = (fun x y -> x <= y);
               eqdec = (fun x y -> x = y) }".
 
+Extract Constant TotalOrder_Project =>
+"fun _ _ -> { compare = (fun x y -> x <= y);
+              eqdec = (fun x y -> x = y) }".
+
+Extract Constant TotalOrder_sum =>
+"fun _ _ -> { compare = (fun x y -> x <= y);
+              eqdec = (fun x y -> x = y) }".
