coq/Extraction/OCaml.v
@@ -27,25 +27,6 @@ Extract Constant exists_last =>
 Extract Constant nth_in_or_default => 
   "fun _ _ _ -> failwith ""nth_in_or_default axiom""".
 
-(** WARNING: risk of overflow, which will generate garbage. *)
-Extract Inductive positive => "int" 
-  [ "(fun n -> 1 + n lsl 1)"
-    "(fun n -> n lsl 1)"  
-    (* most-significant bit is always 1 for positive integers *)
-    "1" ]
-  "(fun lsb1 lsb0 msb1 n ->
-      if n = 1 then msb1 1
-      else if n land 1 = 1 then lsb1 (n lsr 1)
-      else lsb0 (n lsr 1))".
-
-(** WARNING: risk of overflow, which will generate garbage. *)
-Extract Inductive N => "int"
-  [ (* N0  extracts to 0 *) 
-    "0" 
-    (* Npos : positive -> N extracts to positive, which also extracts to int,
-       thus the OCaml code is typable. *)
-    "" ].
-
 (* The generated comparison_rect is a partial function that explodes on
    inputs other than 0, -1, and +1. *)
 Extract Inductive comparison => "int" [ "0" "(-1)" "1" ].
